Tealeaves/Backends/Adapters/Key.v
@@ -1,0 +1,727 @@
+From Tealeaves Require Import
+  Backends.LN.LN
+  Backends.LN.Atom
+  Backends.DB.DB
+  Functors.List
+  Functors.Option
+  Classes.Categorical.ContainerFunctor
+  Classes.Kleisli.DecoratedContainerFunctor.
+
+Open Scope nat_scope.
+
+Import
+  List.ListNotations
+  ContainerFunctor.Notations.
+
+Generalizable All Variables.
+
+(** * Miscellaneous lemmas *)
+(******************************************************************************)
+Lemma nin_list_cons:
+  forall {A : Type} (a1 a2 : A) (xs : list A),
+    ~ a1 ∈ (a2 :: xs) <-> a1 <> a2 /\ ~ a1 ∈ xs.
+Proof.
+  intros. rewrite in_list_cons.
+  intuition.
+Qed.
+
+Lemma map_some: forall `(f: A -> B) (x: option A)  y,
+    (forall a a', f a = f a' -> a = a') ->
+    map f x = Some (f y) ->
+    x = Some y.
+Proof.
+  introv Hinj Heq. destruct x.
+  - inversion Heq. fequal.
+    apply Hinj. assumption.
+  - inversion Heq.
+Qed.
+
+Ltac compare_atoms :=
+    match goal with
+    | H: context[?a == ?a'] |- _ =>
+        destruct_eq_args a a'
+    | |- context[?a == ?a'] =>
+        destruct_eq_args a a'
+    end.
+
+#[global] Tactic Notation "compare" "atoms" := compare_atoms.
+
+(** * Definition of <<key>> and main operations *)
+(******************************************************************************)
+Definition key :=
+  list atom.
+
+(** ** Insertion and lookup *)
+(******************************************************************************)
+Fixpoint key_insert_atom (k: key) (a: atom): key :=
+  match k with
+  | nil => [a]
+  | cons x rest =>
+      if a == x then k else
+        x :: key_insert_atom rest a
+  end.
+
+Fixpoint key_lookup_atom (k: key) (a: atom): option nat :=
+  match k with
+  | [] => None
+  | x :: rest =>
+      if a == x
+      then Some 0
+      else map S (key_lookup_atom rest a)
+  end.
+
+Fixpoint key_lookup_index (k: key) (ix: nat): option atom :=
+  match k, ix with
+  | nil, _ => None
+  | cons a rest, 0 => Some a
+  | cons a rest, S ix => key_lookup_index rest ix
+  end.
+
+Fixpoint key_lookup_atom_rec (k: key) (acc: nat) (a: atom): option nat :=
+  match k with
+  | nil => None
+  | cons x rest =>
+      if a == x then Some acc else key_lookup_atom_rec rest (S acc) a
+  end.
+
+Definition key_lookup_atom_alt: key -> atom -> option nat :=
+  fun k => key_lookup_atom_rec k 0.
+
+(** ** Well-formedness predicates *)
+(******************************************************************************)
+Fixpoint unique (l: list atom): Prop :=
+  match l with
+  | nil => True
+  | cons a rest =>
+      ~ (a ∈ rest) /\ unique rest
+  end.
+
+Definition wf_LN
+  `{Elements T} (t: T LN) (k: key): Prop :=
+  unique k /\ forall (x: atom), Fr x ∈ t -> x ∈ k.
+
+Definition contains_ix_upto (n: nat) (k: key): Prop :=
+  n < length k.
+
+Definition wf_DB `{ElementsCtx nat T} (t: T nat) (k: key): Prop :=
+  unique k /\ exists (gap: nat), closed_gap gap t /\ contains_ix_upto gap k.
+
+(** * Misc *)
+(******************************************************************************)
+Definition key_is_atom_in (k: key) (a: atom):
+  {a ∈ k} + {~ a ∈ k}.
+Proof.
+  induction k.
+  - right. inversion 1.
+  - pose (in_list_cons a a0 k).
+    destruct (a == a0).
+    + now (left; left).
+    + destruct IHk.
+      * now (left; right).
+      * right. rewrite i.
+        intros [contra|contra];
+          contradiction.
+Defined.
+
+Definition key_is_ix_in (k: key) (ix: nat):
+  {contains_ix_upto ix k} + {~ contains_ix_upto ix k}.
+Proof.
+  unfold contains_ix_upto.
+  generalize ix.
+  generalize (length k).
+  intros a b.
+  apply Compare_dec.le_dec.
+Defined.
+
+(** * Lemmas about <<key_insert_atom>> *)
+(******************************************************************************)
+
+(** ** Rewriting *)
+(******************************************************************************)
+Lemma insert_cons_eq: forall a k x,
+    a = x ->
+    key_insert_atom (a :: k) x = a :: k.
+Proof.
+  intros. cbn.
+  destruct_eq_args x a.
+Qed.
+
+Lemma insert_cons_neq: forall a k x,
+    a <> x ->
+    key_insert_atom (a :: k) x = a :: key_insert_atom k x.
+Proof.
+  intros. cbn.
+  destruct_eq_args x a.
+Qed.
+
+(** ** Alternative spec *)
+(******************************************************************************)
+Lemma key_lookup_atom_rec_spec (k: key) (a: atom) (n: nat):
+  key_lookup_atom_rec k n a = map (fun m => m + n) (key_lookup_atom k a).
+Proof.
+  generalize dependent n.
+  induction k; intro n.
+  - reflexivity.
+  - cbn. destruct (a == a0).
+    + reflexivity.
+    + rewrite (IHk (S n)).
+      compose near (key_lookup_atom k a) on right.
+      rewrite (fun_map_map).
+      fequal. ext m. cbn. lia.
+Qed.
+
+Corollary key_lookup_atom_spec (k: key) (a: atom):
+  key_lookup_atom_alt k a = key_lookup_atom k a.
+Proof.
+  unfold key_lookup_atom_alt.
+  rewrite key_lookup_atom_rec_spec.
+  replace (fun m => m + 0) with (@id nat).
+  now rewrite fun_map_id.
+  ext m. unfold id. lia.
+Qed.
+
+(** ** Insertion and <<unique>> *)
+(******************************************************************************)
+Lemma key_nin_insert: forall k a a',
+    a <> a' ->
+    ~ a ∈ k ->
+    ~ a ∈ key_insert_atom k a'.
+Proof.
+  introv Hneq Hnin. induction k.
+  - cbn. intros [H1|H2].
+    + now subst.
+    + assumption.
+  - rewrite nin_list_cons in Hnin.
+    destruct Hnin as [? Hnin].
+    specialize (IHk Hnin).
+    cbn. compare atoms.
+    + intros [contra|contra].
+      now subst. contradiction.
+    + intros [contra|contra].
+      now subst. contradiction.
+Qed.
+
+Theorem key_insert_unique (k: key) (a: atom):
+  unique k ->
+  unique (key_insert_atom k a).
+Proof.
+  intros.
+  induction k.
+  - cbn. easy.
+  - destruct H as [H1 H2].
+    specialize (IHk H2).
+    cbn. compare atoms.
+    cbn. split; auto.
+    apply key_nin_insert; auto.
+Qed.
+
+(** ** Insertion and <<key_lookup_atom>> *)
+(******************************************************************************)
+Lemma key_lookup_atom_not_in1:
+  forall (k:  key) (a: atom),
+    ~ a ∈ k -> key_lookup_atom k a = None.
+Proof.
+  intros. induction k.
+  - reflexivity.
+  - cbn.
+    rewrite nin_list_cons in H.
+    compare atoms.
+    rewrite IHk.
+    + reflexivity.
+    + intuition.
+Qed.
+
+Lemma key_lookup_atom_not_in2:
+  forall (k:  key) (a: atom),
+    key_lookup_atom k a = None -> ~ a ∈ k.
+Proof.
+  intros k a hyp.
+  induction k.
+  - cbv. easy.
+  - rewrite nin_list_cons.
+    cbn in hyp.
+    compare atoms.
+    split.
+    + assumption.
+    + apply IHk.
+      destruct (key_lookup_atom k a).
+      * inversion hyp.
+      * reflexivity.
+Qed.
+
+Theorem key_lookup_atom_not_in_iff:
+  forall (k:  key) (a: atom),
+    ~ a ∈ k <-> key_lookup_atom k a = None.
+Proof.
+  intros. split.
+  - apply key_lookup_atom_not_in1.
+  - apply key_lookup_atom_not_in2.
+Qed.
+
+Lemma key_lookup_atom_in1:
+  forall (k:  key) (a: atom),
+    a ∈ k -> {n: nat | key_lookup_atom k a = Some n}.
+Proof.
+  introv Hin. induction k.
+  - inversion Hin.
+  - rewrite in_list_cons in Hin.
+    cbn. compare atoms.
+    + now (exists 0).
+    + assert (Hink: a ∈ k) by now inversion Hin.
+      destruct (IHk Hink) as [m Hm].
+      rewrite Hm.
+      now (exists (S m)).
+Qed.
+
+Lemma key_lookup_atom_in2:
+  forall (k:  key) (a: atom) (n: nat),
+    key_lookup_atom k a = Some n -> a ∈ k.
+Proof.
+  intros k a.
+  induction k; intros n Heq.
+  - inversion Heq.
+  - rewrite in_list_cons.
+    cbn in Heq.
+    compare atoms.
+    + now left.
+    + right.
+      destruct (key_lookup_atom k a);
+        inversion Heq.
+      now eapply IHk.
+Qed.
+
+Theorem key_lookup_in_atom_iff: forall k a,
+    (exists n, key_lookup_atom k a = Some n) <-> a ∈ k.
+Proof.
+  intros. split.
+  - intros [n H]. eauto using key_lookup_atom_in2.
+  - intro Hin. apply key_lookup_atom_in1 in Hin.
+    firstorder.
+Qed.
+
+Theorem key_lookup_atom_decide:
+  forall (k: key) (a: atom),
+    ((a ∈ k) * {n: nat | key_lookup_atom k a = Some n}) +
+      {~ a ∈ k /\ key_lookup_atom k a = None}.
+Proof.
+  intros.
+  destruct (key_is_atom_in k a); [left|right].
+  - split.
+    + assumption.
+    + auto using key_lookup_atom_in1.
+  - split.
+    + assumption.
+    + auto using key_lookup_atom_not_in1.
+Defined.
+
+Ltac lookup_atom_in_key k a :=
+  let n := fresh "n" in
+  let Hin := fresh "H_in" in
+  let Hnin := fresh "H_not_in" in
+  destruct (key_lookup_atom_decide k a) as
+    [[Hin [n H_key_lookup]] | [Hnin H_key_lookup]];
+  try contradiction.
+
+Tactic Notation "lookup" "atom" constr(a) "in" "key" constr(k) :=
+  lookup_atom_in_key k a.
+
+Goal forall k (a: atom), a ∈ k \/ ~ a ∈ k.
+Proof.
+  intros.
+  lookup atom a in key k.
+  - left. intuition.
+  - now right.
+Qed.
+
+Lemma key_lookup_atom_cons_0: forall a a' k,
+    key_lookup_atom (a :: k) a' = Some 0 ->
+    a = a'.
+Proof.
+  introv Hlookup; cbn in *.
+  compare atoms.
+  lookup atom a' in key k;
+    rewrite H_key_lookup in Hlookup;
+    now inversion Hlookup.
+Qed.
+
+Lemma key_lookup_atom_cons_S: forall a x k ix,
+    key_lookup_atom (x :: k) a = Some (S ix) ->
+    a <> x /\ key_lookup_atom k a = Some ix.
+Proof.
+  introv HH.
+  cbn in HH.
+  destruct_eq_args a x.
+  split. assumption.
+  eauto using (map_some S).
+Qed.
+
+Theorem key_lookup_atom_cons: forall a k a' ix,
+    key_lookup_atom (a :: k) a' = Some ix ->
+    (a' = a /\ ix = 0) \/
+      (a' <> a /\ exists ix', ix = S ix' /\ key_lookup_atom k a' = Some ix').
+Proof.
+  introv Hyp. destruct ix; [left|right].
+  - apply key_lookup_atom_cons_0 in Hyp.
+    intuition.
+  - apply key_lookup_atom_cons_S in Hyp.
+    intuition eauto.
+Qed.
+
+(** ** Insertion and <<key_lookup_ix>> *)
+(******************************************************************************)
+Lemma key_lookup_ix_in:
+  forall (k:  key) (ix: nat) (a: atom),
+    key_lookup_index k ix = Some a -> a ∈ k.
+Proof.
+  introv Hin.
+  generalize dependent ix.
+  induction k; intros ix Hin.
+  - inversion Hin.
+  - destruct ix.
+    + cbn in *. inversion Hin. now left.
+    + cbn in Hin.
+      rewrite in_list_cons.
+      right. eauto.
+Qed.
+
+Lemma key_lookup_ix_Some1:
+  forall (k:  key) (ix: nat) (a: atom),
+    key_lookup_index k ix = Some a -> contains_ix_upto ix k.
+Proof.
+  introv Hin.
+  unfold contains_ix_upto.
+  generalize dependent ix.
+  induction k; intros ix Hin.
+  - false.
+  - destruct ix.
+    + cbn. lia.
+    + cbn. cbn in Hin.
+      specialize (IHk ix Hin).
+      lia.
+Qed.
+
+Lemma key_lookup_ix_Some2:
+  forall (k:  key) (ix: nat),
+    contains_ix_upto ix k ->
+    {a:atom | key_lookup_index k ix = Some a}.
+Proof.
+  unfold contains_ix_upto.
+  intros.
+  generalize dependent k.
+  induction ix; intros k Hlt.
+  - destruct k.
+    + cbn in Hlt. lia.
+    + cbn. eauto.
+  - destruct k.
+    + false. cbn in Hlt. lia.
+    + cbn in Hlt.
+      cbn.
+      specialize (IHix k ltac:(lia)).
+      assumption.
+Qed.
+
+Lemma key_lookup_ix_Some_iff:
+  forall (k:  key) (ix: nat),
+    contains_ix_upto ix k <->
+      exists a, key_lookup_index k ix = Some a.
+Proof.
+  intros. split.
+  - intro H; apply key_lookup_ix_Some2 in H. firstorder.
+  - intros [a H]. eapply key_lookup_ix_Some1. eauto.
+Qed.
+
+Lemma key_lookup_ix_None1:
+  forall (k:  key) (ix: nat),
+    key_lookup_index k ix = None -> ~ (contains_ix_upto ix k).
+Proof.
+  introv Hin.
+  unfold contains_ix_upto.
+  generalize dependent ix.
+  induction k; intros ix Hin.
+  - cbn. lia.
+  - destruct ix.
+    + false.
+    + cbn. cbn in Hin.
+      specialize (IHk ix Hin).
+      apply PeanoNat.Nat.le_ngt.
+      lia.
+Qed.
+
+Lemma key_lookup_ix_None2:
+  forall (k:  key) (ix: nat),
+    ~ (contains_ix_upto ix k) ->
+    key_lookup_index k ix = None.
+Proof.
+  introv Hin.
+  unfold contains_ix_upto in *.
+  generalize dependent ix.
+  induction k; intros ix Hin.
+  - reflexivity.
+  - cbn in *. destruct ix.
+    + contradict Hin. lia.
+    + specialize (IHk ix ltac:(lia)).
+      assumption.
+Qed.
+
+Theorem key_lookup_ix_decide:
+  forall (k: key) (n: nat),
+    ((contains_ix_upto n k) * {a: atom | key_lookup_index k n = Some a}) +
+      {~ contains_ix_upto n k /\ key_lookup_index k n = None}.
+Proof.
+  intros.
+  destruct (key_is_ix_in k n); [left|right].
+  - split.
+    + assumption.
+    + auto using key_lookup_ix_Some2.
+  - split.
+    + assumption.
+    + auto using key_lookup_ix_None2.
+Defined.
+
+Ltac lookup_ix_in_key k n :=
+  let a := fresh "a" in
+  let Hcont := fresh "Hcont" in
+  let H_key_lookup := fresh "H_key_lookup" in
+  destruct (key_lookup_ix_decide k n) as
+    [[Hcont [a H_key_lookup]] | [Hcont H_key_lookup]];
+  try contradiction.
+
+Tactic Notation "lookup" "index" constr(ix) "in" "key" constr(k) :=
+  lookup_ix_in_key k ix.
+
+Goal forall k (ix: nat), contains_ix_upto ix k \/ ~ contains_ix_upto ix k.
+Proof.
+  intros.
+  lookup index ix in key k.
+  - left. intuition.
+  - now right.
+Qed.
+
+(** ** Properties of <<get_index>> *)
+(******************************************************************************)
+(*
+Lemma get_index_rec_S (acc: nat) (a: atom) (k: key):
+  get_index_rec (S acc) a k = map S (get_index_rec acc a k).
+Proof.
+  generalize dependent acc.
+  induction k; intro.
+  - cbn. reflexivity.
+  - cbn. destruct_eq_args a a0.
+Qed.
+
+Lemma get_index_rec_plus (acc acc': nat) (a: atom) (k: key):
+  get_index_rec (acc + acc') a k =
+    map (fun acc => acc + acc') (get_index_rec acc a k).
+Proof.
+  generalize dependent acc.
+  induction k; intro.
+  - cbn. reflexivity.
+  - cbn. destruct_eq_args a a0.
+    rewrite get_index_rec_S.
+    rewrite IHk.
+    rewrite get_index_rec_S.
+    compose near (get_index_rec acc a k).
+    rewrite (fun_map_map).
+    rewrite (fun_map_map).
+    reflexivity.
+Qed.
+
+Lemma get_index_rec_plus_Some1 (acc acc': nat) (a: atom) (k: key) (ix: nat):
+  get_index_rec acc a k = Some ix ->
+    get_index_rec (acc + acc') a k = Some (ix + acc').
+Proof.
+  introv hyp.
+  rewrite get_index_rec_plus.
+  rewrite hyp.
+  reflexivity.
+Qed.
+
+Lemma get_index_rec_plus_Some2 (acc acc': nat) (a: atom) (k: key) (ix: nat):
+  get_index_rec (acc + acc') a k = Some (ix + acc') ->
+  get_index_rec acc a k = Some ix.
+Proof.
+  rewrite get_index_rec_plus.
+  apply (map_some (fun x => x + acc')).
+  intros n m. lia.
+Qed.
+ *)
+
+(** *** Keys known to contain a particular element *)
+(******************************************************************************)
+(*
+Lemma get_index_rec_in (acc: nat) (x: atom) (k: key):
+  x ∈ k -> exists ix, get_index_rec acc x k = Some ix.
+Proof.
+  intros.
+  induction k.
+  - false.
+  - cbn. destruct_eq_args x a.
+    + eauto.
+    + autorewrite with tea_list in H.
+      destruct H; [false|].
+      specialize (IHk H).
+      rewrite get_index_rec_S.
+      destruct IHk as [ix hyp].
+      exists (S ix).
+      rewrite hyp.
+      reflexivity.
+Qed.
+
+Corollary get_index_in (x: atom) (k: key):
+  x ∈ k -> exists ix, get_index x k = Some ix.
+Proof.
+  unfold get_index.
+  apply get_index_rec_in.
+Qed.
+
+Lemma get_index_rec_insert1 (acc: nat) (a: atom) (k: key) (x: atom):
+  a = x ->
+  exists (m: nat), get_index_rec acc a (key_insert_atom k x) = Some m.
+Proof.
+  intro Heq.
+  subst.
+  generalize dependent acc.
+  induction k; intro acc.
+  - cbn. destruct_eq_args x x. exists acc. reflexivity.
+  - destruct (x == a).
+    + subst. rewrite (insert_cons_eq a _ a Logic.eq_refl).
+      cbn. destruct_eq_args a a. eauto.
+    + rewrite insert_cons_neq. cbn.
+      destruct_eq_args x a. eauto.
+Qed.
+
+Corollary get_index_insert1 (a: atom) (k: key) (x: atom):
+  a = x ->
+  exists (m: nat), get_index a (insert k x) = Some m.
+Proof.
+  apply get_index_rec_insert1.
+Qed.
+
+
+Lemma get_atom_rw2: forall a k ix,
+    key_lookup_atom_rec (a :: k) (S ix) =
+      key_lookup_atom_rec k ix.
+Proof.
+  intros.
+  cbn.
+  reflexivity.
+Qed.
+
+Lemma get_index_rec_neqS: forall a k n,
+    n > 0 ->
+    get_index_rec n a k <> Some 0.
+Proof.
+  intros.
+  generalize dependent n.
+  induction k; introv hyp.
+  - cbn. easy.
+  - cbn.
+    specialize (IHk (S n) ltac:(lia)).
+    destruct (a == a0).
+    + inversion 1. lia.
+    + assumption.
+Qed.
+
+Lemma get_index_Some_0: forall a x k,
+    get_index a (x :: k) = Some 0 <->
+      a = x.
+Proof.
+  introv.
+  cbn.
+  destruct_eq_args a x.
+  split.
+  - intro contra.
+    apply get_index_rec_neqS in contra.
+    false. lia.
+  - inversion 1. false.
+Qed.
+
+*)
+
+(** ** Properties of <<key_lookup_index>> *)
+(******************************************************************************)
+Lemma key_lookup_zero: forall a k ix,
+    ix = 0 ->
+    key_lookup_index (a :: k) ix = Some a.
+Proof.
+  intros. subst.
+  reflexivity.
+Qed.
+
+(*
+Lemma map_key_lookup_atom_Z: forall k a,
+    map S (key_lookup_atom_alt k a) = Some 0 -> False.
+Proof.
+  intros.
+  destruct (key_lookup_atom_alt k a).
+  - cbn in H. inversion H.
+  - inversion H.
+Qed.
+ *)
+
+Lemma key_lookup_index_S: forall k ix a,
+    key_lookup_index k ix = Some a ->
+    forall a', key_lookup_index (a' :: k) (S ix) = Some a.
+Proof.
+  intros.
+  assumption.
+Qed.
+
+Lemma key_lookup_index_cons: forall a' a k ix,
+    key_lookup_index (a' :: k) ix = Some a ->
+    ix = 0 /\ a = a' \/
+      exists ix', ix = S ix' /\ key_lookup_index k ix' = Some a.
+Proof.
+  introv Hin. destruct ix.
+  - cbn in Hin. inversion Hin.
+    left. now split.
+  - cbn in Hin. right.
+    exists ix. split; auto.
+Qed.
+
+Lemma key_bijection1: forall a k ix,
+    key_lookup_atom k a = Some ix ->
+    key_lookup_index k ix = Some a.
+Proof.
+  intros.
+  generalize dependent ix.
+  induction k; intros ix Hix.
+  - cbn in *. inversion Hix.
+  - apply key_lookup_atom_cons in Hix.
+    destruct Hix as
+      [ [Heq Hix0] | [Hneq [Hix [Heq Hlookup]]] ]; subst.
+    + reflexivity.
+    + cbn. auto.
+Qed.
+
+Lemma key_bijection2: forall a k ix,
+    unique k ->
+    key_lookup_index k ix = Some a ->
+    key_lookup_atom k a = Some ix.
+Proof.
+  introv Huniq Hix.
+  generalize dependent ix.
+  induction k; intros ix Hix.
+  - cbn in Hix. inversion Hix.
+  - cbn.
+    apply key_lookup_index_cons in Hix.
+    destruct Hix as [[Hix_zero Heq] | [ix' [Heq Hrest]]].
+    + subst. compare atoms.
+    + destruct Huniq as [Hnin Huniq].
+      specialize (IHk Huniq).
+      compare atoms.
+      * false.
+        apply key_lookup_ix_in in Hrest.
+        contradiction.
+      * rewrite (IHk ix' Hrest).
+        reflexivity.
+Qed.
+
+Lemma key_bijection: forall a k ix,
+    unique k ->
+    key_lookup_index k ix = Some a <->
+      key_lookup_atom k a = Some ix.
+Proof.
+  intros.
+  split; auto using key_bijection1, key_bijection2.
+Qed.
